First Part of correctnes of Inject

TM/Inject.v
@@ -1,27 +1,26 @@
 Require Import Prelim Relations TM Shared.Tactics.AutoIndTac Compound.
+Require Import TM.Relations.
 
-Fixpoint inject m n Z (indices : Vector.t ((Fin.t m)) n) (def : Z) (V : Vector.t Z n) : Vector.t Z m.
+Fixpoint inject m n Z (indices : Vector.t ((Fin.t n)) m) (def : Z) (V : Vector.t Z m) : Vector.t Z n.
 Proof.
   destruct indices.
-  - eapply (Vector.const def).
-  - remember (S n) as Sn. destruct V eqn:E; inversion HeqSn; subst.
+  - apply (Vector.const def).
+  - rename n0 into m. remember (S m) as Sn. destruct V eqn:E; inversion HeqSn; subst.
     pose (x := inject _ _ _ indices def t).
     exact (Vector.replace x h h0).
 Defined.
 
-
 Inductive dupfree X : forall n, Vector.t X n -> Prop :=
   dupfreeVN : dupfree (@Vector.nil X)
 | dupfreeVC n (x : X) (V : Vector.t X n) : ~ Vector.In x V -> dupfree V -> (dupfree (x ::: V))%vector_scope.
-
 
 Lemma Vector_nth_In (X : Type) (n : nat) (p : Fin.t n) (m : nat) (new_pos : X) (V : Vector.t X n) :
     V[@p] = new_pos -> Vector.In (new_pos) V.
 Proof.
   intros. induction V;dependent destruct p; cbn in *; subst; econstructor; eauto.
 Qed.
-  
-Lemma inject_correct_Some m n Z (indices : Vector.t ((Fin.t m)) n) (def : Z) (V : Vector.t Z n) pos new_pos :
+
+Lemma inject_correct_Some m n Z (indices : Vector.t (Fin.t n) m) (def : Z) (V : Vector.t Z m) pos new_pos :
   dupfree indices ->
   indices[@pos] = new_pos -> V[@pos] = (inject indices def V) [@new_pos].
 Proof.
@@ -35,6 +34,67 @@ Proof.
       * erewrite Vector_replace_nth2; eauto.
 Qed.
 
+Lemma inject_correct m n Z (indices : Vector.t (Fin.t n) m) (def : Z) (V : Vector.t Z m) :
+  dupfree indices -> reorder indices (inject indices def V) = V.
+Proof.
+  intros H. unfold reorder. apply Vector.eq_nth_iff. intros p ? <-.
+  erewrite Vector.nth_map; eauto. erewrite <- inject_correct_Some; eauto.
+Qed.
+  
+Section Map_Algebra.
+  
+  Lemma typecheck (m n : nat) (A I X Y Z : Type)
+        (x : Vector.t X n) (y : Vector.t Y n) (i : Vector.t I m)
+        (f : Vector.t A n -> I -> Z)
+        (g : X -> Y -> A) :
+    Vector.map (f (Vector.map2 g x y)) i =
+    Vector.map (f (Vector.map2 g x y)) i.
+  Abort.
+
+  Lemma map_map (A B I : Type) (n : nat) (g : A -> B)  (f : I -> A) (i : Vector.t I n) :
+    Vector.map g (Vector.map f i) = Vector.map (fun x => g (f x)) i.
+  Proof.
+    general induction i.
+    - reflexivity.
+    - cbn. f_equal. auto.
+  Qed.
+
+  Lemma map_eq (n : nat) (A B : Type) (f1 f2 : A -> B) (x : Vector.t A n) :
+    (forall k : Fin.t n, f1 (x[@k]) = f2 (x[@k])) ->
+    Vector.map f1 x = Vector.map f2 x.
+  Proof.
+    intros H. apply Vector.eq_nth_iff. intros k ? <-.
+    erewrite Vector.nth_map. erewrite Vector.nth_map.
+    apply H. reflexivity. reflexivity.
+  Qed.
+
+  Lemma map_map_nth (A X : Type) (m n : nat)
+        (g : X -> A)
+        (x : Vector.t X m)
+        (i : Vector.t (Fin.t m) n) :
+    Vector.map (Vector.nth (Vector.map g x)) i =
+    Vector.map g (Vector.map (Vector.nth x) i).
+  Proof.
+    rewrite map_map. apply map_eq. intros k. now apply Vector.nth_map.
+  Qed.
+
+  Lemma map2_map_nth (A X Y : Type) (m n : nat)
+        (g : X -> Y -> A)
+        (x : Vector.t X n)
+        (y : Vector.t Y n)
+        (i : Vector.t (Fin.t n) m) :
+    Vector.map (Vector.nth (Vector.map2 g x y)) i =
+    Vector.map2 g
+                (Vector.map (Vector.nth x) i)
+                (Vector.map (Vector.nth y) i).
+  Proof.
+    apply Vector.eq_nth_iff. intros k ? <-.
+    erewrite !Vector.nth_map2; eauto. erewrite !Vector.nth_map; eauto. erewrite !Vector.nth_map2; eauto.
+  Qed.
+  
+End Map_Algebra.
+
+    
 Section Injection.
 
   Variable sig : finType.
@@ -46,74 +106,84 @@ Section Injection.
   Variable pM : { M : mTM sig m & states M -> F}.
 
   Variable I : Vector.t ((Fin.t (S n))) (S m).
-  Definition M := projT1 pM.
+  Variable I_dupfree : dupfree I.
 
   Definition trans_inj :=
     fun '(q, sym ) =>
-      let (q', act) := trans (m := M) (q, reorder I sym) in
+      let (q', act) := trans (m := projT1 pM) (q, reorder I sym) in
       (q', inject I (None, N) act).
 
   Definition injectM : mTM sig n.
   Proof.
     econstructor.
     exact trans_inj.
-    exact (start M).
-    exact (halt (m := M)).
+    exact (start (projT1 pM)).
+    exact (halt (m := projT1 pM)).
   Defined.
 
   Definition Inject := (injectM; projT2 pM).
 
   Ltac double H := let H' := fresh H in assert (H' := H).
 
-  Lemma sim q q' t t' t2 t2' :
-    perm I t t2 ->
-    perm I t' t2' ->
-    step (M := M) (mk_mconfig q t) = mk_mconfig q' t' <->
-    step (M := injectM) (mk_mconfig q t2) = mk_mconfig q' t2'.
-  Proof.
-    Require Import Coq.Program.Equality.
-  Admitted.
-      
-    
 
-    
+
+  Lemma sim_step (c1 c2 : mconfig sig (states (projT1 pM)) n) :
+    step (M := injectM) c1 = c2 ->
+    step (M := projT1 pM) (mk_mconfig (cstate c1) (reorder I (ctapes c1))) =
+    (mk_mconfig (cstate c2) (reorder I (ctapes c2))).
+  Proof.
+    intros H.
+    Set Printing Implicit.
+    unfold injectM in *.
+    Unset Printing Implicit.
+    destruct c1 as [state1 tapes1] eqn:E1, c2 as [state2 tapes2] eqn:E2.
+    unfold step in *. cbn in *.
+    unfold reorder in *. cbn in *.
+
+    destruct (trans
+                (state1,
+                 Vector.map (Vector.nth (Vector.map (current (sig:=sig)) tapes1)) I))
+             as (q, act) eqn:E3.
+    injection H; clear H; intros H1 H2; subst.
+
+    destruct (trans (state1, Vector.map (current (sig:=sig)) (Vector.map (Vector.nth tapes1) I)))
+             as (q', act') eqn:E4.
+
+    enough ((state2, act) = (q', act')) as X.
+    {
+      inv X. f_equal.
+      rewrite map2_map_nth. f_equal.
+      symmetry. pose proof inject_correct as Lemma. unfold reorder in Lemma. now apply Lemma.
+    }
+    rewrite <- E3, <- E4. f_equal. f_equal. now apply map_map_nth.
+  Qed.
+
+  Lemma sim_loop (c1 c2 : mconfig sig (states (projT1 pM)) n) (i : nat) :
+    loopM (M := injectM) i c1 = Some c2 ->
+    loopM (M := projT1 pM) i (mk_mconfig (cstate c1) (reorder I (ctapes c1))) =
+    Some (mk_mconfig (cstate c2) (reorder I (ctapes c2))).
+  Proof.
+    unfold loopM in *. general induction i; cbn in *.
+    - destruct (halt _) eqn:E; now inv H.
+    - destruct (halt _) eqn:E; inv H; try rewrite E in *; auto.
+      rewrite sim_step with (c2 := step (M := injectM) c1); auto.
+  Qed.
+  
   Lemma Inject_sem (R : Rel (tapes sig (S m)) (F * tapes sig (S m))) :
     pM ⊫ R ->
     Inject ⊫ lift_gen_eq_p I R.
   Proof.
-    intros ***.
-    general induction i.
-    - double H0.
-      cbn in H0.
-      destruct (halt (start M)) eqn:E; inv H0.
-      cbn. firstorder. unfold lift_gen_p. cbn in H1.      
-      eapply (H (reorder I t) 0 (initc M (reorder I t))).
-      cbn. unfold M in *; destruct _; now inv H1.
+    intros H.
+    split.
+    - apply (H (reorder I t) i (mk_mconfig (cstate outc) (reorder I (ctapes outc)))).
+      pose proof (@sim_loop (initc injectM t) outc i) as Lemma. cbn in Lemma. now apply Lemma.
+    - 
   Admitted.
 
   Lemma Inject_term T :
-    M ↓ T ->
+    projT1 pM ↓ T ->
     projT1 Inject ↓ liftT_gen I T.
   Proof.
   Admitted.
 
-End 
-
-
-
-
-
-
-
-
-
-
-
-
-
-
-
-
-
-
-  
+End.
